Lemmas.v
@@ -1,7 +1,5 @@
 From Coq Require Import Arith ZArith Psatz Bool String List Program.Equality.
 
-Ltac inv H := inversion H; clear H; subst.
-
 Lemma Zge_refl: forall (n: Z), (n >= n)%Z.
 intros. lia. Qed.
 
@@ -21,3 +19,47 @@ Proof.
   destruct (ge_diff Hge) as [k Hk].
   exists k; assumption.
 Qed.
+
+(* COMPCERT *)
+Ltac inv H := inversion H; clear H; subst.
+
+Lemma modusponens: forall (P Q: Prop), P -> (P -> Q) -> Q.
+Proof. auto. Qed.
+
+Ltac exploit x :=
+    refine (modusponens _ _ (x _ _ _ _ _ _ _ _ _ _ _ _ _ _ _ _ _ _ _ _ _ _ _ _ _ _ _ _ _ _ _ _ _ _ _) _)
+ || refine (modusponens _ _ (x _ _ _ _ _ _ _ _ _ _ _ _ _ _ _ _ _ _ _ _ _ _ _ _ _ _ _ _ _ _ _ _ _ _) _)
+ || refine (modusponens _ _ (x _ _ _ _ _ _ _ _ _ _ _ _ _ _ _ _ _ _ _ _ _ _ _ _ _ _ _ _ _ _ _ _ _) _)
+ || refine (modusponens _ _ (x _ _ _ _ _ _ _ _ _ _ _ _ _ _ _ _ _ _ _ _ _ _ _ _ _ _ _ _ _ _ _ _) _)
+ || refine (modusponens _ _ (x _ _ _ _ _ _ _ _ _ _ _ _ _ _ _ _ _ _ _ _ _ _ _ _ _ _ _ _ _ _ _) _)
+ || refine (modusponens _ _ (x _ _ _ _ _ _ _ _ _ _ _ _ _ _ _ _ _ _ _ _ _ _ _ _ _ _ _ _ _ _) _)
+ || refine (modusponens _ _ (x _ _ _ _ _ _ _ _ _ _ _ _ _ _ _ _ _ _ _ _ _ _ _ _ _ _ _ _ _) _)
+ || refine (modusponens _ _ (x _ _ _ _ _ _ _ _ _ _ _ _ _ _ _ _ _ _ _ _ _ _ _ _ _ _ _ _) _)
+ || refine (modusponens _ _ (x _ _ _ _ _ _ _ _ _ _ _ _ _ _ _ _ _ _ _ _ _ _ _ _ _ _ _) _)
+ || refine (modusponens _ _ (x _ _ _ _ _ _ _ _ _ _ _ _ _ _ _ _ _ _ _ _ _ _ _ _ _ _) _)
+ || refine (modusponens _ _ (x _ _ _ _ _ _ _ _ _ _ _ _ _ _ _ _ _ _ _ _ _ _ _ _ _) _)
+ || refine (modusponens _ _ (x _ _ _ _ _ _ _ _ _ _ _ _ _ _ _ _ _ _ _ _ _ _ _ _) _)
+ || refine (modusponens _ _ (x _ _ _ _ _ _ _ _ _ _ _ _ _ _ _ _ _ _ _ _ _ _ _) _)
+ || refine (modusponens _ _ (x _ _ _ _ _ _ _ _ _ _ _ _ _ _ _ _ _ _ _ _ _ _) _)
+ || refine (modusponens _ _ (x _ _ _ _ _ _ _ _ _ _ _ _ _ _ _ _ _ _ _ _ _) _)
+ || refine (modusponens _ _ (x _ _ _ _ _ _ _ _ _ _ _ _ _ _ _ _ _ _ _ _) _)
+ || refine (modusponens _ _ (x _ _ _ _ _ _ _ _ _ _ _ _ _ _ _ _ _ _ _) _)
+ || refine (modusponens _ _ (x _ _ _ _ _ _ _ _ _ _ _ _ _ _ _ _ _ _) _)
+ || refine (modusponens _ _ (x _ _ _ _ _ _ _ _ _ _ _ _ _ _ _ _ _) _)
+ || refine (modusponens _ _ (x _ _ _ _ _ _ _ _ _ _ _ _ _ _ _ _) _)
+ || refine (modusponens _ _ (x _ _ _ _ _ _ _ _ _ _ _ _ _ _ _) _)
+ || refine (modusponens _ _ (x _ _ _ _ _ _ _ _ _ _ _ _ _ _) _)
+ || refine (modusponens _ _ (x _ _ _ _ _ _ _ _ _ _ _ _ _) _)
+ || refine (modusponens _ _ (x _ _ _ _ _ _ _ _ _ _ _ _) _)
+ || refine (modusponens _ _ (x _ _ _ _ _ _ _ _ _ _ _) _)
+ || refine (modusponens _ _ (x _ _ _ _ _ _ _ _ _ _) _)
+ || refine (modusponens _ _ (x _ _ _ _ _ _ _ _ _) _)
+ || refine (modusponens _ _ (x _ _ _ _ _ _ _ _) _)
+ || refine (modusponens _ _ (x _ _ _ _ _ _ _) _)
+ || refine (modusponens _ _ (x _ _ _ _ _ _) _)
+ || refine (modusponens _ _ (x _ _ _ _ _) _)
+ || refine (modusponens _ _ (x _ _ _ _) _)
+ || refine (modusponens _ _ (x _ _ _) _)
+ || refine (modusponens _ _ (x _ _) _)
+ || refine (modusponens _ _ (x _) _).
+
